hacking on sketch, define _to_deep functions, prove is_in stuff

sketchScript.sml
@@ -1,9 +1,52 @@
 open HolKernel boolLib bossLib lcsymtacs
-open pred_setTheory
-open holSemanticsTheory
+open miscLib stringSyntax listSyntax pred_setTheory
+open setSpecTheory holSemanticsTheory
 
 val _ = temp_tight_equality()
 val _ = new_theory"sketch"
+
+(* TODO: use mk_syntax_fns *)
+
+local open String in
+fun tyvar_to_deep s =
+  if sub(s,0) = #"'" then
+    if size s = 2 then str(Char.toUpper (sub(s,1)))
+    else extract(s,1,NONE)
+  else s
+end
+
+val type_ty = ``:type``
+
+fun type_to_deep ty =
+  if is_type ty then
+    case dest_thy_type ty of { Args = args, Thy = thy, Tyop = tyop } =>
+      let
+        val name = fromMLstring tyop
+        val args = List.map type_to_deep args
+        val args = mk_list(args,type_ty)
+      in
+        ``Tyapp ^name ^args``
+      end
+  else
+    let
+      val name = dest_vartype ty
+      val name = tyvar_to_deep name
+      val name = fromMLstring name
+    in
+      ``Tyvar ^name``
+    end
+
+fun term_to_deep tm =
+  case dest_term tm of
+    VAR(x,ty) => ``Var ^(fromMLstring x) ^(type_to_deep ty)``
+  | CONST {Name,Thy,Ty} => ``Const ^(fromMLstring Name) ^(type_to_deep Ty)``
+  | COMB (f,x) => ``Comb ^(term_to_deep f) ^(term_to_deep x)``
+  | LAMB (x,b) =>
+      let
+        val (x,ty) = dest_var x
+      in
+        ``Abs ^(fromMLstring x) ^(type_to_deep ty) ^(term_to_deep b)``
+      end
 
 val mem = ``mem:'U->'U->bool``
 
@@ -22,21 +65,124 @@ val in_bool_def = Define`
   in_bool0 ^mem = Boolean`
 val _ = Parse.overload_on("in_bool",``in_bool0 ^mem``)
 
-(*
-val in_bool_is_bij = store_thm("in_bool_is_bij",
-  ``is_set_theory ^mem ==> BIJ in_bool UNIV (ext (range in_bool))``,
-  rw[in_bool_def,ext_def,range_def,BIJ_IFF_INV] >- (
+val is_in_def = Define`
+  is_in0 ^mem f = ∃x. BIJ f UNIV {a | mem a x}`
+val _ = Parse.overload_on("is_in",``is_in0 ^mem``)
 
-    rw[in_bool_def,boolean_in_boolset] ) >>
+val is_in_in_bool = store_thm("is_in_in_bool",
+  ``is_set_theory ^mem ⇒
+    is_in in_bool``,
+  rw[is_in_def,BIJ_IFF_INV] >>
+  qexists_tac`boolset` >>
+  rw[in_bool_def,boolean_in_boolset] >>
   qexists_tac`λx. x = True` >>
   rw[in_bool_def,boolean_eq_true] >>
   rfs[mem_boolset,boolean_eq_true,true_neq_false,boolean_def])
-*)
 
 val in_fun_def = Define`
   in_fun0 ^mem ina inb f =
     Abstract (range ina) (range inb) (λx. inb (f (finv ina x)))`
 val _ = Parse.overload_on("in_fun",``in_fun0 ^mem``)
+
+val out_fun_def = Define`
+  out_fun0 ^mem ina inb mf x = finv inb (mf ' (ina x))`
+val _ = Parse.overload_on("out_fun",``out_fun0 ^mem``)
+
+val is_in_range_thm = store_thm("is_in_range_thm",
+  ``∀f. is_in f ⇒ BIJ f UNIV (ext (range f))``,
+  rw[is_in_def,range_def] >>
+  SELECT_ELIM_TAC >> conj_tac >- metis_tac[] >>
+  rw[ext_def])
+
+val is_in_finv_left = store_thm("is_in_finv_left",
+  ``∀ina.
+    is_in ina ⇒ ∀x. finv ina (ina x) = x``,
+  rw[finv_def] >>
+  SELECT_ELIM_TAC >>
+  conj_tac >-metis_tac[] >>
+  fs[is_in_def,BIJ_DEF,INJ_DEF])
+
+val is_in_finv_right = store_thm("is_in_finv_right",
+  ``∀ina.
+    is_in ina ⇒ ∀x. x <: range ina ⇒
+      (ina (finv ina x)) = x``,
+  rw[finv_def] >>
+  SELECT_ELIM_TAC >>
+  conj_tac >-(
+    imp_res_tac is_in_range_thm >>
+    fs[ext_def,BIJ_DEF,SURJ_DEF] ) >>
+  rw[])
+
+val is_in_in_fun = store_thm("is_in_in_fun",
+  ``is_set_theory ^mem ⇒
+    ∀ina inb. is_in ina ∧ is_in inb ⇒ is_in (in_fun ina inb)``,
+  rw[] >>
+  rw[is_in_def,BIJ_IFF_INV] >>
+  qexists_tac`Funspace (range ina) (range inb)` >>
+  conj_tac >- (
+    rw[in_fun_def] >>
+    match_mp_tac (UNDISCH abstract_in_funspace) >>
+    simp[range_def] >>
+    SELECT_ELIM_TAC >>
+    conj_tac >- metis_tac[is_in_def] >>
+    rw[] >>
+    SELECT_ELIM_TAC >>
+    conj_tac >- metis_tac[is_in_def] >>
+    rw[] >>
+    fs[BIJ_IFF_INV] ) >>
+  qexists_tac`out_fun ina inb` >>
+  conj_tac >- (
+    rw[out_fun_def,in_fun_def,FUN_EQ_THM] >>
+    qmatch_abbrev_tac`finv invb (Abstract s t f ' a) = Z` >>
+    rfs[] >>
+    `Abstract s t f ' a = f a` by (
+      match_mp_tac (UNDISCH apply_abstract) >>
+      imp_res_tac is_in_range_thm >>
+      fs[ext_def,BIJ_IFF_INV] >>
+      unabbrev_all_tac >> fs[] ) >>
+    rw[Abbr`Z`,Abbr`f`,Abbr`a`,Abbr`invb`] >>
+    imp_res_tac is_in_finv_left >>
+    simp[] ) >>
+  rw[in_fun_def,out_fun_def] >>
+  first_x_assum(mp_tac o
+    MATCH_MP(REWRITE_RULE[GSYM AND_IMP_INTRO](UNDISCH in_funspace_abstract))) >>
+  simp[AND_IMP_INTRO] >>
+  discharge_hyps >- (
+    imp_res_tac is_in_range_thm >>
+    fs[ext_def,BIJ_IFF_INV] >>
+    metis_tac[] ) >>
+  rw[] >>
+  match_mp_tac (UNDISCH abstract_eq) >>
+  gen_tac >>
+  qspecl_then[`f`,`ina (finv ina x)`,`range ina`,`range inb`]mp_tac
+    (UNDISCH apply_abstract) >>
+  discharge_hyps >- (
+    imp_res_tac is_in_range_thm >>
+    fs[ext_def,BIJ_DEF,INJ_DEF] ) >>
+  rw[] >>
+  imp_res_tac is_in_finv_right >>
+  rw[])
+
+val base_tysig_def = Define`
+  base_tysig = FEMPTY |++ [("fun",2);("bool",0)]`
+val base_tmsig_def = Define`
+  base_tmsig = FEMPTY |++ [("=",Fun (Tyvar "A") (Tyvar "A"))]`
+
+val P = ``x:bool``
+val tysig = ``base_tysig``
+val tmsig = ``base_tmsig``
+
+val thm = prove(
+  ``is_set_theory ^mem ∧
+    is_interpretation (^tysig,^tmsig) (tyass,tmass) ∧
+    is_std_interpretation (tyass,tmass) ∧
+    is_valuation ^tysig tmass (tyval,tmval) ∧
+    tmval ("x",Bool) = in_bool x
+    ⇒
+    in_bool x =
+      termsem ^tmsig (tyass,tmass) (tyval,tmval) (Var "x" Bool)``,
+  rw[termsem_def])
+
 
 (*
 P = ``ARB (c:α->β) (x:ind->ind) (ARB:α list)``
@@ -102,6 +248,5 @@ fun mk_in (ty : hol_type) =
         mk_in_var ty
   else
     mk_in_var ty
- 
 
 val _ = export_theory()
